src/Std/Data/DHashMap/Internal/RawLemmas.lean
@@ -71,6 +71,7 @@ variable [BEq α] [Hashable α]
 scoped macro "wf_trivial" : tactic => `(tactic|
   repeat (first
     | apply Raw₀.wfImp_insert | apply Raw₀.wfImp_insertIfNew | apply Raw₀.wfImp_erase
+    | apply Raw₀.wfImp_alter | apply Raw₀.wfImp_modify
     | apply Raw.WF.out | assumption | apply Raw₀.wfImp_empty | apply Raw.WFImp.distinct
     | apply Raw.WF.empty₀))
 
@@ -90,7 +91,8 @@ private def queryNames : Array Name :=
     ``Raw.pairwise_keys_iff_pairwise_keys]
 
 private def modifyNames : Array Name :=
-  #[``toListModel_insert, ``toListModel_erase, ``toListModel_insertIfNew]
+  #[``toListModel_insert, ``toListModel_erase, ``toListModel_insertIfNew, ``toListModel_alter,
+    ``toListModel_modify]
 
 private def congrNames : MacroM (Array (TSyntax `term)) := do
   return #[← `(_root_.List.Perm.isEmpty_eq), ← `(containsKey_of_perm),
@@ -123,6 +125,15 @@ theorem isEmpty_empty {c} : (empty c : Raw₀ α β).1.isEmpty := by
 theorem isEmpty_insert [EquivBEq α] [LawfulHashable α] (h : m.1.WF) {k : α} {v : β k} :
     (m.insert k v).1.isEmpty = false := by
   simp_to_model using List.isEmpty_insertEntry
+
+@[simp]
+theorem isEmpty_modify [LawfulBEq α] (h : m.1.WF) {k : α} {f : β k → β k} :
+    (m.modify k f).1.isEmpty ↔ m.1.isEmpty := by
+  simp_to_model using List.isEmpty_modifyKey
+
+theorem isEmpty_alter [LawfulBEq α] (h : m.1.WF) {k : α} {f : Option (β k) → Option (β k)} :
+    (m.alter k f).1.isEmpty ↔ (m.erase k).1.isEmpty ∧ f (m.get? k) = none := by
+  simp_to_model using List.isEmpty_alterKey
 
 theorem contains_congr [EquivBEq α] [LawfulHashable α] (h : m.1.WF) {a b : α} (hab : a == b) :
     m.contains a = m.contains b := by
