src/Std/Data/DHashMap/Internal/WF.lean
@@ -543,6 +543,12 @@ theorem toListModel_alterₘ [BEq α] [Hashable α] [LawfulBEq α] {m : Raw₀ �
       rw [insertEntry_of_containsKey_eq_false]
       exact hc
 
+theorem toListModel_alter [BEq α] [Hashable α] [LawfulBEq α] {m : Raw₀ α β} (h : Raw.WFImp m.1)
+    {a : α} {f : Option (β a) → Option (β a)} :
+    Perm (toListModel (m.alter a f).1.2) (alterKey a f (toListModel m.1.2)) := by
+  rw [alter_eq_alterₘ]
+  exact toListModel_alterₘ h
+
 theorem wfImp_alterₘ [BEq α] [Hashable α] [LawfulBEq α] {m : Raw₀ α β} (h : Raw.WFImp m.1) {a : α}
     {f : Option (β a) → Option (β a)} : Raw.WFImp (m.alterₘ a f).1 where
   buckets_hash_self := isHashSelf_alterₘ m h a f
@@ -591,18 +597,18 @@ theorem isHashSelf_updateBucket_alter [BEq α] [EquivBEq α] [Hashable α] [Lawf
   rw [AssocList.Const.toList_alter.mem_iff] at hp
   by_cases h : p.fst == a
   · exact .inr <| hash_eq h
-  · rw [mem_alterKey_of_key_ne _ h] at hp
+  · rw [Const.mem_alterKey_of_key_not_beq _ h] at hp
     exact .inl <| containsKey_of_mem hp
 
-theorem wfImp_updateBucket_alter [BEq α] [Hashable α] {m : Raw₀ α (fun _ => β)}
+theorem wfImp_updateBucket_alter [BEq α] [EquivBEq α] [Hashable α] [LawfulHashable α] {m : Raw₀ α (fun _ => β)}
     (h : Raw.WFImp m.1) {a : α} {f : Option β → Option β} :
     Raw.WFImp (withComputedSize <| updateBucket m.1.buckets m.2 a (AssocList.Const.alter a f)) where
   buckets_hash_self := isHashSelf_updateBucket_alter h
   size_eq := by rw [size_withComputedSize, computeSize_eq]; rfl
-  distinct := DistinctKeys.perm (toListModel_updateBucket_alter h) h.distinct.alterKey
+  distinct := DistinctKeys.perm (toListModel_updateBucket_alter h) h.distinct.constAlterKey
 
-theorem isHashSelf_alterₘ [BEq α] [Hashable α] (m : Raw₀ α (fun _ => β)) (h : Raw.WFImp m.1)
-    (a : α) (f : Option β → Option β) : IsHashSelf (m.alterₘ a f).1.buckets := by
+theorem isHashSelf_alterₘ [BEq α] [EquivBEq α] [Hashable α] [LawfulHashable α] (m : Raw₀ α (fun _ => β)) (h : Raw.WFImp m.1)
+    (a : α) (f : Option β → Option β) : IsHashSelf (Const.alterₘ m a f).1.buckets := by
   dsimp only [alterₘ, withComputedSize]
   split
   · exact isHashSelf_updateBucket_alter h
@@ -612,15 +618,15 @@ theorem isHashSelf_alterₘ [BEq α] [Hashable α] (m : Raw₀ α (fun _ => β))
     · refine (wfImp_expandIfNecessary _ (wfImp_consₘ _ h _ _ ?_)).buckets_hash_self
       exact Bool.not_eq_true _ ▸ hc
 
-theorem toListModel_alterₘ [BEq α] [Hashable α] {m : Raw₀ α (fun _ => β)} (h : Raw.WFImp m.1)
+theorem toListModel_alterₘ [BEq α] [EquivBEq α] [Hashable α] [LawfulHashable α] {m : Raw₀ α (fun _ => β)} (h : Raw.WFImp m.1)
     {a : α} {f : Option β → Option β} :
-    Perm (toListModel (m.alterₘ a f).1.2) (alterKey a f (toListModel m.1.2)) := by
-  rw [alterₘ]
+    Perm (toListModel (Const.alterₘ m a f).1.2) (Const.alterKey a f (toListModel m.1.2)) := by
+  rw [Const.alterₘ]
   split
   · exact toListModel_updateBucket_alter h
   · next hc =>
     rw [Bool.not_eq_true, containsₘ_eq_containsKey h] at hc
-    rw [alterKey, getValueCast?_eq_none hc]
+    rw [Const.alterKey, getValue?_eq_none.mpr hc]
     split
     · next hn =>
       simp only [hn]
@@ -633,39 +639,45 @@ theorem toListModel_alterₘ [BEq α] [Hashable α] {m : Raw₀ α (fun _ => β)
       rw [insertEntry_of_containsKey_eq_false]
       exact hc
 
-theorem wfImp_alterₘ [BEq α] [Hashable α] {m : Raw₀ α (fun _ => β)} (h : Raw.WFImp m.1) {a : α}
-    {f : Option β → Option β} : Raw.WFImp (m.alterₘ a f).1 where
+theorem wfImp_alterₘ [BEq α] [EquivBEq α] [Hashable α] [LawfulHashable α] {m : Raw₀ α (fun _ => β)} (h : Raw.WFImp m.1) {a : α}
+    {f : Option β → Option β} : Raw.WFImp (Const.alterₘ m a f).1 where
   buckets_hash_self := isHashSelf_alterₘ m h a f
-  distinct := DistinctKeys.perm (toListModel_alterₘ h) h.distinct.alterKey
+  distinct := DistinctKeys.perm (toListModel_alterₘ h) h.distinct.constAlterKey
   size_eq := by
     rw [← Perm.length_eq (toListModel_alterₘ h).symm, alterₘ]
     split
     · next h₁ =>
       rw [containsₘ_eq_containsKey h] at h₁
-      simp only [length_alterKey, h.size_eq, dif_pos h₁]
+      simp only [Const.length_alterKey, h.size_eq, dif_pos h₁]
       rw [containsₘ_eq_containsKey (by apply wfImp_updateBucket_alter h)]
       simp only [buckets_withComputedSize]
       simp only [containsKey_of_perm <| toListModel_updateBucket_alter h]
-      rw [← getValueCast?_eq_some_getValueCast h₁]
-      conv => lhs; congr; rw [containsKey_alterKey_iff (a := a) (f := f) h.distinct];
+      rw [← getValue?_eq_some_getValue h₁]
+      conv => lhs; congr; rw [Const.containsKey_alterKey_iff (a := a) (f := f) h.distinct];
     · next h₁ =>
       rw [containsₘ_eq_containsKey h] at h₁
-      rw [alterKey]
-      rw [getValueCast?_eq_none <| Bool.not_eq_true _ ▸ h₁]
+      rw [Const.alterKey]
+      rw [getValue?_eq_none.mpr <| Bool.not_eq_true _ ▸ h₁]
       split
       · next heq =>
         rw [heq, h.size_eq, length_eraseKey, if_neg h₁]
       · next heq =>
         rw [heq, size_expandIfNecessary, consₘ, length_insertEntry, if_neg h₁, h.size_eq]
 
-theorem wfImp_alter [BEq α] [Hashable α] {m : Raw₀ α (fun _ => β)}
-    (h : Raw.WFImp m.1) {a : α} {f : Option β → Option β} : Raw.WFImp (m.alter a f).1 := by
-  rw [alter_eq_alterₘ]
+theorem wfImp_alter [BEq α] [EquivBEq α] [Hashable α] [LawfulHashable α] {m : Raw₀ α (fun _ => β)}
+    (h : Raw.WFImp m.1) {a : α} {f : Option β → Option β} : Raw.WFImp (Const.alter m a f).1 := by
+  rw [Const.alter_eq_alterₘ]
   exact wfImp_alterₘ h
 
 end Const
 
 /-! # `modify` -/
+
+theorem toListModel_modify [BEq α] [Hashable α] [LawfulBEq α] {m : Raw₀ α β} (h : Raw.WFImp m.1)
+    {a : α} {f : β a → β a} :
+    Perm (toListModel (m.modify a f).1.2) (modifyKey a f (toListModel m.1.2)) := by
+  rw [modify_eq_alter, modifyKey_eq_alterKey]
+  exact toListModel_alter h
 
 theorem wfImp_modifyₘ [BEq α] [Hashable α] [LawfulBEq α] {m : Raw₀ α β}
     (h : Raw.WFImp m.1) {a : α} {f : β a → β a} : Raw.WFImp (m.modifyₘ a f).1 := wfImp_alterₘ h
@@ -679,12 +691,12 @@ namespace Const
 
 variable {β : Type v}
 
-theorem wfImp_modifyₘ [BEq α] [Hashable α] {m : Raw₀ α (fun _ => β)}
-    (h : Raw.WFImp m.1) {a : α} {f : β → β} : Raw.WFImp (m.modifyₘ a f).1 := wfImp_alterₘ h
+theorem wfImp_modifyₘ [BEq α] [EquivBEq α] [Hashable α] [LawfulHashable α] {m : Raw₀ α (fun _ => β)}
+    (h : Raw.WFImp m.1) {a : α} {f : β → β} : Raw.WFImp (Const.modifyₘ m a f).1 := Const.wfImp_alterₘ h
 
-theorem wfImp_modify [BEq α] [Hashable α] {m : Raw₀ α (fun _ => β)} (h : Raw.WFImp m.1) {a : α}
-    {f : β → β} : Raw.WFImp (m.modify a f).1 := by
-  rw [modify_eq_modifyₘ]
+theorem wfImp_modify [BEq α] [EquivBEq α] [Hashable α] [LawfulHashable α] {m : Raw₀ α (fun _ => β)} (h : Raw.WFImp m.1) {a : α}
+    {f : β → β} : Raw.WFImp (Const.modify m a f).1 := by
+  rw [Const.modify_eq_modifyₘ]
   exact wfImp_alterₘ h
 
 end Const
@@ -958,10 +970,10 @@ theorem WF.out [BEq α] [Hashable α] [i₁ : EquivBEq α] [i₂ : LawfulHashabl
   · next h => exact Raw₀.wfImp_filter (by apply h)
   · next h => exact Raw₀.Const.wfImp_getThenInsertIfNew? (by apply h)
   · next h => exact Raw₀.wfImp_modify (by apply h)
-  · next h => exact Raw₀.wfImp_constModify (by apply h)
+  · next h => exact Raw₀.Const.wfImp_modify (by apply h)
     done
   · next h => exact Raw₀.wfImp_alter (by apply h)
-  · next h => exact Raw₀.wfImp_constAlter (by apply h)
+  · next h => exact Raw₀.Const.wfImp_alter (by apply h)
 
 end Raw
 
